ToClean.lean
@@ -16,5 +16,6 @@ import ToClean.Circuit.StaticTable
 import ToClean.Air.TableBuild
 import ToClean.Air.UnitBalance
 import ToClean.Air.TransitionView
+import ToClean.Air.ReceiverView
 import ToClean.Air.MessageFilter
 import ToClean.Tactic.GetElemFastPath
